state/TargetLang.fst
@@ -3,376 +3,48 @@ module TargetLang
 open FStar.Tactics
 open FStar.Tactics.Typeclasses
 
-open Labeled.Monotonic.Heap
-open Labeled.MST
+open SharedRefs
 open Witnessable
-
-type inv_typ =
-  | InvT_Unit
-  | InvT_Nat
-  | InvT_Sum : inv_typ -> inv_typ -> inv_typ
-  | InvT_Pair : inv_typ -> inv_typ -> inv_typ
-  | InvT_Ref : inv_typ -> inv_typ
-  | InvT_LList : inv_typ -> inv_typ
-
-let rec to_Type (t:inv_typ) : Type u#0 = 
-  match t with
-  | InvT_Unit -> unit
-  | InvT_Nat -> int
-  | InvT_Sum t1 t2 -> either (to_Type t1) (to_Type t2)
-  | InvT_Pair t1 t2 -> (to_Type t1) * (to_Type t2)
-  | InvT_Ref t -> ref (to_Type t)
-  | InvT_LList t -> linkedList (to_Type t)
-
-let rec to_Type_solve (t:inv_typ) : witnessable (to_Type t) =
-  match t with
-  | InvT_Unit -> witnessable_unit
-  | InvT_Nat -> witnessable_int
-  | InvT_Sum t1 t2 -> witnessable_sum (to_Type t1) (to_Type t2) #(to_Type_solve t1) #(to_Type_solve t2)
-  | InvT_Pair t1 t2 -> witnessable_pair (to_Type t1) (to_Type t2) #(to_Type_solve t1) #(to_Type_solve t2)
-  | InvT_Ref t -> witnessable_ref (to_Type t) #(to_Type_solve t)
-  | InvT_LList t -> witnessable_llist (to_Type t) #(to_Type_solve t)
-
-let inv_points_to (h:lheap) pred =
-  // forall (a:Type) (c:witnessable a) (r:ref a). 
-  //   (witnessable_ref _ #c).satisfy r h pred ==>
-  //     c.satisfy (sel h r) h pred
-  // CA: previous version does not work because in proofs, one needs to prove a property like:
-  // forall (a:Type) (c:witnessable a) (c':witnessable a) (r:ref a).
-  //   c.satisfy r h pred ==> c'.satisfy r h pred
-
-  // however, the following version needs an inversion lemma that cannot be proven in F* yet
-  // because one cannot reason about the types of effectful arrows. e.g., `int =!= int -> ST int` cannot be proven
-  (forall (a:inv_typ) (r:ref (to_Type a)).
-    (witnessable_ref _ #(to_Type_solve a)).satisfy r h pred ==> 
-      (to_Type_solve a).satisfy (sel h r) h pred)
-
-let inv_low_contains (h:lheap) = 
-  inv_points_to h contains_pred /\ inv_points_to h is_low_pred
-
-let eliminate_inv_points_to (h:lheap) a (r:ref (to_Type a)) pred :
-  Lemma
-    (requires (inv_points_to h pred))
-    (ensures (
-      (witnessable_ref (to_Type a) #(to_Type_solve a)).satisfy r h pred ==> 
-        (to_Type_solve a).satisfy (sel h r) h pred
-    )) = ()
-
-let eliminate_inv_low h a (r:ref (to_Type a)) :
-  Lemma
-    (requires (inv_points_to h is_low_pred))
-    (ensures (
-      (witnessable_ref (to_Type a) #(to_Type_solve a)).satisfy r h is_low_pred ==> 
-        (to_Type_solve a).satisfy (sel h r) h is_low_pred
-    )) = ()
-
-let eliminate_inv_contains h a (hinv:lheap -> Type0) (r:ref (to_Type a)) :
-  Lemma
-    (requires (inv_points_to h contains_pred))
-    (ensures (
-      (witnessable_ref (to_Type a) #(to_Type_solve a)).satisfy r h contains_pred ==> 
-        (to_Type_solve a).satisfy (sel h r) h contains_pred
-    )) = ()
-
-let rec inversion (a:inv_typ) (xa:inv_typ) :
-  Lemma
-    (requires (to_Type a == to_Type xa))
-    (ensures (a == xa /\ to_Type_solve a == to_Type_solve xa)) =
-  match a with
-  | InvT_Unit -> ()
-  | InvT_Nat -> ()
-  | InvT_Sum t1 t2 -> begin
-    let InvT_Sum t1' t2' = xa in
-    assume (forall a b c d. either a b == either c d ==> a == c /\ b == d);
-    inversion t1 t1';
-    inversion t2 t2'
-  end
-  | InvT_Pair t1 t2 -> begin
-    let InvT_Pair t1' t2' = xa in
-    assume (forall a b c d. (a * b) == (c * d) ==> a == c /\ b == d);
-    inversion t1 t1';
-    inversion t2 t2'
-  end
-  | InvT_Ref t -> begin
-    let InvT_Ref t' = xa in
-    assume (forall a b. ref a == ref b ==> a == b);
-    inversion t t'
-  end
-  | InvT_LList t -> begin
-    let InvT_LList t' = xa in
-    assume (forall a b. linkedList a == linkedList b ==> a == b);
-    inversion t t'
-  end
-  
-let lemma_write_preserves_is_low t (x:ref (to_Type t)) (v:to_Type t) (h0 h1:lheap) : Lemma
-  (requires (
-    h0 `lheap_rel` h1 /\
-    equal_dom h0 h1 /\
-    modifies (Set.singleton (addr_of x)) h0 h1 /\
-    modifies_classification Set.empty h0 h1 /\
-    sel h1 x == v /\
-    (to_Type_solve (InvT_Ref t)).satisfy x h0 is_low_pred /\
-    (to_Type_solve t).satisfy v h0 is_low_pred /\
-    inv_points_to h0 is_low_pred))
-  (ensures (
-    inv_points_to h1 is_low_pred)) = 
-  introduce forall a (r:ref (to_Type a)).
-      (witnessable_ref _ #(to_Type_solve a)).satisfy r h1 is_low_pred ==> 
-        (to_Type_solve a).satisfy (sel h1 r) h1 is_low_pred
-  with begin
-    introduce (witnessable_ref _ #(to_Type_solve a)).satisfy r h1 is_low_pred 
-      ==> (to_Type_solve a).satisfy (sel h1 r) h1 is_low_pred
-    with _. begin
-      introduce addr_of r =!= addr_of x ==> (to_Type_solve a).satisfy (sel h1 r) h1 is_low_pred with _. begin
-        eliminate_inv_points_to h0 a r is_low_pred;
-        (to_Type_solve a).satisfy_monotonic (sel h0 r) is_low_pred h0 h1
-      end;
-      introduce addr_of r == addr_of x ==> (to_Type_solve a).satisfy (sel h1 r) h1 is_low_pred with _. begin
-        assert (sel h1 x == v);
-        lemma_sel_same_addr' h1 x r;
-        inversion a t;
-        assert ((to_Type_solve t).satisfy v h0 is_low_pred);
-        (to_Type_solve t).satisfy_monotonic v is_low_pred h0 h1;
-        assert ((to_Type_solve t).satisfy v h1 is_low_pred)
-      end
-    end
-  end
-
-let lemma_write_preserves_contains t (x:ref (to_Type t)) (v:to_Type t) (h0 h1:lheap) : Lemma
-  (requires (
-    h0 `lheap_rel` h1 /\
-    equal_dom h0 h1 /\
-    modifies (Set.singleton (addr_of x)) h0 h1 /\
-    modifies_classification Set.empty h0 h1 /\
-    sel h1 x == v /\
-    (to_Type_solve (InvT_Ref t)).satisfy x h0 contains_pred /\
-    (to_Type_solve t).satisfy v h0 contains_pred /\
-    inv_points_to h0 contains_pred))
-  (ensures (
-    inv_points_to h1 contains_pred)) = 
-  introduce forall a (r:ref (to_Type a)).
-      (witnessable_ref _ #(to_Type_solve a)).satisfy r h1 contains_pred ==> 
-        (to_Type_solve a).satisfy (sel h1 r) h1 contains_pred
-  with begin
-    introduce (witnessable_ref _ #(to_Type_solve a)).satisfy r h1 contains_pred 
-      ==> (to_Type_solve a).satisfy (sel h1 r) h1 contains_pred
-    with _. begin
-      introduce addr_of r =!= addr_of x ==> (to_Type_solve a).satisfy (sel h1 r) h1 contains_pred with _. begin
-        eliminate_inv_points_to h0 a r contains_pred;
-        (to_Type_solve a).satisfy_monotonic (sel h0 r) contains_pred h0 h1
-      end;
-      introduce addr_of r == addr_of x ==> (to_Type_solve a).satisfy (sel h1 r) h1 contains_pred with _. begin
-        assert (sel h1 x == v);
-        lemma_sel_same_addr' h1 x r;
-        inversion a t;
-        assert ((to_Type_solve t).satisfy v h0 contains_pred);
-        (to_Type_solve t).satisfy_monotonic v contains_pred h0 h1;
-        assert ((to_Type_solve t).satisfy v h1 contains_pred)
-      end
-    end
-  end
-
-
-let lemma_declassify_preserves_contains t (x:ref (to_Type t)) (h0 h1:lheap) : Lemma
-  (requires (
-    modifies_none h0 h1 /\
-    h0 `lheap_rel` h1 /\
-    equal_dom h0 h1 /\
-    modifies_classification (only x) h0 h1 /\
-    (to_Type_solve (InvT_Ref t)).satisfy x h0 contains_pred /\ 
-    (to_Type_solve t).satisfy (sel h0 x) h0 contains_pred /\
-    inv_points_to h0 contains_pred))
-  (ensures (inv_points_to h1 contains_pred)) =
-  introduce forall a (r:ref (to_Type a)).
-      (witnessable_ref _ #(to_Type_solve a)).satisfy r h1 contains_pred ==> 
-        (to_Type_solve a).satisfy (sel h1 r) h1 contains_pred
-  with begin
-    let refw = witnessable_ref _ #(to_Type_solve a) in
-    introduce refw.satisfy r h1 contains_pred ==> (to_Type_solve a).satisfy (sel h1 r) h1 contains_pred
-    with _. begin
-      introduce refw.satisfy r h0 contains_pred ==> (to_Type_solve a).satisfy (sel h1 r) h1 contains_pred
-      with _. (to_Type_solve a).satisfy_monotonic (sel h0 r) contains_pred h0 h1;
-      
-      introduce ~(refw.satisfy r h0 contains_pred) ==> (to_Type_solve a).satisfy (sel h1 r) h1 contains_pred
-      with _. begin
-        assert (addr_of r == addr_of x);
-        lemma_sel_same_addr' h1 x r;
-        assert (to_Type_solve a == to_Type_solve t);
-        inversion a t;
-        assert (to_Type_solve a == to_Type_solve t);
-
-        assert ((to_Type_solve t).satisfy (sel h0 x) h0 contains_pred);
-        (to_Type_solve t).satisfy_monotonic (sel h0 x) contains_pred h0 h1;
-        assert (sel h0 x == sel h1 x);
-        assert ((to_Type_solve t).satisfy (sel h1 x) h1 contains_pred);
-        assert ((to_Type_solve a).satisfy (sel h1 r) h1 contains_pred)
-      end
-    end
-  end
-
-let lemma_declassify_preserves_is_low t (x:ref (to_Type t)) (h0 h1:lheap) : Lemma
-  (requires (
-    modifies_none h0 h1 /\
-    h0 `lheap_rel` h1 /\
-    equal_dom h0 h1 /\
-    modifies_classification (only x) h0 h1 /\
-    (to_Type_solve (InvT_Ref t)).satisfy x h1 is_low_pred /\
-    (to_Type_solve t).satisfy (sel h0 x) h0 is_low_pred /\
-    inv_points_to h0 is_low_pred))
-  (ensures (inv_points_to h1 is_low_pred)) =
-  introduce forall a (inv:lheap -> Type0) (r:ref (to_Type a)).
-      (witnessable_ref _ #(to_Type_solve a)).satisfy r h1 is_low_pred ==> 
-        (to_Type_solve a).satisfy (sel h1 r) h1 is_low_pred
-  with begin
-    let refw = witnessable_ref _ #(to_Type_solve a) in
-    introduce refw.satisfy r h1 is_low_pred ==> (to_Type_solve a).satisfy (sel h1 r) h1 is_low_pred
-    with _. begin
-      introduce refw.satisfy r h0 is_low_pred ==> (to_Type_solve a).satisfy (sel h1 r) h1 is_low_pred
-      with _. (to_Type_solve a).satisfy_monotonic (sel h0 r) is_low_pred h0 h1;
-      
-      introduce ~(refw.satisfy r h0 is_low_pred) ==> (to_Type_solve a).satisfy (sel h1 r) h1 is_low_pred
-      with _. begin
-        assert (addr_of r == addr_of x);
-        lemma_sel_same_addr' h1 x r;
-        inversion a t;
-        (to_Type_solve t).satisfy_monotonic (sel h0 x) is_low_pred h0 h1
-      end
-    end
-  end
-
-let lemma_ist_alloc_preserves_contains t (x:ref (to_Type t)) (v:to_Type t) (h0 h1:lheap) : Lemma
-  (requires (
-    h0 `lheap_rel` h1 /\
-    h1 == upd h0 x v /\ 
-    fresh x h0 h1 /\ 
-    modifies Set.empty h0 h1 /\
-    modifies_classification Set.empty h0 h1 /\
-    sel h1 x == v /\ 
-    label_of x h1 == High /\
-    is_mm x == false /\
-    (to_Type_solve t).satisfy v h0 contains_pred /\
-    inv_points_to h0 contains_pred))
-  (ensures (
-    inv_points_to h1 contains_pred)) = 
-  introduce forall a (r:ref (to_Type a)).
-      (witnessable_ref _ #(to_Type_solve a)).satisfy r h1 contains_pred ==> 
-        (to_Type_solve a).satisfy (sel h1 r) h1 contains_pred
-  with begin
-    introduce (witnessable_ref _ #(to_Type_solve a)).satisfy r h1 contains_pred 
-      ==> (to_Type_solve a).satisfy (sel h1 r) h1 contains_pred
-    with _. begin
-      introduce addr_of r =!= addr_of x ==> (to_Type_solve a).satisfy (sel h1 r) h1 contains_pred with _. begin
-        eliminate_inv_points_to h0 a r contains_pred;
-        assert (h0 `contains` r);
-        (to_Type_solve a).satisfy_monotonic (sel h0 r) contains_pred h0 h1
-      end;
-      introduce addr_of r == addr_of x ==> (to_Type_solve a).satisfy (sel h1 r) h1 contains_pred with _. begin
-        assert (sel h1 x == v);
-        lemma_sel_same_addr' h1 x r;
-        inversion a t;
-        (to_Type_solve t).satisfy_monotonic v contains_pred h0 h1
-      end
-    end
-  end
-
-let lemma_ist_alloc_preserves_is_low t (x:ref (to_Type t)) (v:to_Type t) (h0 h1:lheap) : Lemma
-  (requires (
-    h0 `lheap_rel` h1 /\
-    h1 == upd h0 x v /\ 
-    fresh x h0 h1 /\ 
-    modifies Set.empty h0 h1 /\
-    modifies_classification Set.empty h0 h1 /\
-    sel h1 x == v /\ 
-    label_of x h1 == High /\
-    is_mm x == false /\
-    (to_Type_solve t).satisfy v h0 contains_pred /\
-    inv_points_to h0 is_low_pred))
-  (ensures (
-    inv_points_to h1 is_low_pred)) = 
-  introduce forall a (r:ref (to_Type a)).
-      (witnessable_ref _ #(to_Type_solve a)).satisfy r h1 is_low_pred ==> 
-        (to_Type_solve a).satisfy (sel h1 r) h1 is_low_pred
-  with begin
-    introduce (witnessable_ref _ #(to_Type_solve a)).satisfy r h1 is_low_pred 
-      ==> (to_Type_solve a).satisfy (sel h1 r) h1 is_low_pred
-    with _. begin
-      introduce addr_of r =!= addr_of x ==> (to_Type_solve a).satisfy (sel h1 r) h1 is_low_pred with _. begin
-        eliminate_inv_points_to h0 a r is_low_pred;
-        assert (h0 `contains` r);
-        (to_Type_solve a).satisfy_monotonic (sel h0 r) is_low_pred h0 h1;
-        assert ((to_Type_solve a).satisfy (sel h1 r) h1 is_low_pred)
-      end;
-      introduce addr_of r == addr_of x ==> (to_Type_solve a).satisfy (sel h1 r) h1 is_low_pred with _. begin
-        assert (sel h1 x == v);
-        lemma_sel_same_addr' h1 x r;
-        assert (label_of r h1 == Low);
-        assert (label_of x h1 == High);
-        assert (r == x);
-        assert False
-      end
-    end
-  end
-
-
-effect IST (a:Type) (pre:st_pre) (post: (h:lheap -> Tot (st_post' a (pre h)))) =
-  ST a 
-    (requires (fun h0      -> inv_low_contains h0 /\ pre h0))
-    (ensures  (fun h0 r h1 -> inv_low_contains h1 /\ post h0 r h1))
-
-
-let ist_alloc (#t:inv_typ) (init:to_Type t)
-: IST (ref (to_Type t))
-    (fun h -> 
-      (to_Type_solve t).satisfy init h contains_pred)
-    (alloc_post #(to_Type t) init)
-=
-  let h0 = get () in
-  let r = alloc init in
-  let h1 = get () in
-  lemma_ist_alloc_preserves_contains t r init h0 h1;
-  lemma_ist_alloc_preserves_is_low t r init h0 h1;
-  r
-
 
 open STLC
 
-let rec to_inv_typ (t:typ0) : inv_typ =
+let rec to_shareable_typ (t:typ0) : shareable_typ =
   match t with
-  | TUnit -> InvT_Unit
-  | TNat -> InvT_Nat
-  | TSum t1 t2 -> InvT_Sum (to_inv_typ t1) (to_inv_typ t2)
-  | TPair t1 t2 -> InvT_Pair (to_inv_typ t1) (to_inv_typ t2)
-  | TRef t -> InvT_Ref (to_inv_typ t)
-  | TLList t -> InvT_LList (to_inv_typ t)
-
-(** elab_typ0 should be in translation file, but it is here because 
-    we need it to write our invariants **)
+  | TUnit -> SUnit
+  | TNat -> SNat
+  | TSum t1 t2 -> SSum (to_shareable_typ t1) (to_shareable_typ t2)
+  | TPair t1 t2 -> SPair (to_shareable_typ t1) (to_shareable_typ t2)
+  | TRef t -> SRef (to_shareable_typ t)
+  | TLList t -> SLList (to_shareable_typ t)
 
 unfold
 let elab_typ0 (t:typ0) : Type u#0 = 
-  to_Type (to_inv_typ t)
+  to_Type (to_shareable_typ t)
 
-unfold
-let elab_typ0_tc (t:typ0) : witnessable (elab_typ0 t) =
-  to_Type_solve (to_inv_typ t)
-
-unfold let shallowly_contained_low (#a:Type) (v:a) {| c:witnessable a |} (h:lheap) =
-  c.satisfy v h contains_pred /\ c.satisfy v h is_low_pred
+let rec elab_typ0_tc (t:typ0) : witnessable (elab_typ0 t) = 
+  match t with
+  | TUnit -> witnessable_unit
+  | TNat -> witnessable_int
+  | TSum t1 t2 -> witnessable_sum _ _ #(elab_typ0_tc t1) #(elab_typ0_tc t2)
+  | TPair t1 t2 -> witnessable_pair _ _ #(elab_typ0_tc t1) #(elab_typ0_tc t2)
+  | TRef t -> witnessable_ref _ #(elab_typ0_tc t) 
+  | TLList t -> witnessable_llist _ #(elab_typ0_tc t)
 
 unfold let pre_tgt_arrow
   (#t1:Type) {| c1 : witnessable t1 |}
-  (x:t1) (h0:lheap) =
-  inv_low_contains h0 /\
-  shallowly_contained_low x #c1 h0
+  (x:t1) =
+  sst_pre (fun h0 ->
+    c1.satisfy x h0 contains_pred /\
+    c1.satisfy x h0 shareS.is_shared)
 
 unfold let post_tgt_arrow
   (#t1:Type) {| c1 : witnessable t1 |}
   (#t2:Type) {| c2 : witnessable t2 |}
-  (x:t1) (h0:lheap) (r:t2) (h1:lheap) =
-  inv_low_contains h1 /\
-  modifies_only_label Low h0 h1 /\                       (* allows low references to be modified *)
-  modifies_classification Set.empty h0 h1 /\             (* no modifications of the classification *)
-  shallowly_contained_low r #c2 h1
+  (x:t1) =
+  sst_post t2 (pre_tgt_arrow #t1 #c1 x) (fun h0 r h1 -> 
+    modifies_only_shared h0 h1 /\     (* allows shared references to be modified and to alloc new reference and share them *)
+    c2.satisfy r h1 contains_pred /\
+    c2.satisfy r h1 shareS.is_shared)
 
 let mk_tgt_arrow
   (t1:Type) {| c1 : witnessable t1 |}
@@ -380,6 +52,40 @@ let mk_tgt_arrow
 = x:t1 -> ST t2 
     (requires (pre_tgt_arrow #t1 #c1 x ))
     (ensures (post_tgt_arrow #t1 #c1 #t2 #c2 x))
+
+let rec lemma_123 (#t:typ0) (v:elab_typ0 t) h pred :
+  Lemma ((elab_typ0_tc t).satisfy v h pred <==> forallRefsHeap pred h #(to_shareable_typ t) v) 
+  // [SMTPat ((elab_typ0_tc t).satisfy v h pred); SMTPat (forallRefsHeap pred h #(to_shareable_typ t) v)]
+  by (compute ()) =
+  match t with
+  | TUnit -> ()
+  | TNat -> ()
+  | TSum t1 t2 -> begin
+    let v : either (elab_typ0 t1) (elab_typ0 t2) = v in
+    match v with
+    | Inl lv -> lemma_123 lv h pred
+    | Inr rv -> lemma_123 rv h pred
+  end
+  | TPair t1 t2 -> begin
+     let v : (elab_typ0 t1) * (elab_typ0 t2) = v in
+     lemma_123 (fst v) h pred;
+     lemma_123 (snd v) h pred;
+     assert ((elab_typ0_tc t).satisfy v h pred <==> forallRefsHeap pred h #(to_shareable_typ t) v)
+  end
+  | TRef t' -> 
+    let aux (#t':typ0) (v:elab_typ0 (TRef t')) : ref (elab_typ0 t') = v in
+    let v : ref (elab_typ0 t') = aux v in
+    assert ((elab_typ0_tc t).satisfy v h pred <==> forallRefsHeap pred h #(to_shareable_typ t) v) by (compute ())
+  | TLList t' -> begin
+    let aux (#t':typ0) (v:elab_typ0 (TLList t')) : linkedList (elab_typ0 t') = v in
+    let v : linkedList (elab_typ0 t') = aux v in
+    match v with
+    | LLNil -> ()
+    | LLCons v' xsref -> (
+      lemma_123 v' h pred;
+      let xsref : ref (linkedList (elab_typ0 t')) = xsref in
+      assert ((elab_typ0_tc t).satisfy v h pred <==> forallRefsHeap pred h #(to_shareable_typ t) v))
+  end
 
 open FStar.Universe
 
@@ -389,7 +95,7 @@ let rec _elab_typ (t:typ) : tt:Type u#1 & witnessable tt =
     let tt1 = _elab_typ t1 in
     let tt2 = _elab_typ t2 in
     (| mk_tgt_arrow (dfst tt1) #(dsnd tt1) (dfst tt2) #(dsnd tt2),
-       witnessable_arrow (dfst tt1) (dfst tt2) pre_tgt_arrow post_tgt_arrow
+       witnessable_arrow (dfst tt1) (dfst tt2) (pre_tgt_arrow) (post_tgt_arrow)
     |)
   end 
   | TUnit -> (| raise_t unit, solve |)
@@ -417,130 +123,46 @@ let elab_typ (t:typ) : Type =
 let elab_typ_tc (t:typ) : witnessable (elab_typ t) =
   dsnd (_elab_typ t)
 
-let eliminate_inv_low' h (a:typ0) (r:ref (elab_typ0 a)) :
-  Lemma
-    (requires (inv_points_to h is_low_pred))
-    (ensures (
-      (witnessable_ref _ #(elab_typ0_tc a)).satisfy r h is_low_pred ==> 
-        (elab_typ0_tc a).satisfy (sel h r) h is_low_pred
-    )) = eliminate_inv_low h (to_inv_typ a) r
-
-let eliminate_inv_contains' (h:lheap) (a:typ0) (r:ref (elab_typ0 a)) :
-  Lemma
-    (requires (inv_points_to h contains_pred))
-    (ensures (
-      (witnessable_ref _ #(elab_typ0_tc a)).satisfy r h contains_pred ==> 
-        (elab_typ0_tc a).satisfy (sel h r) h contains_pred
-    )) = eliminate_inv_contains h (to_inv_typ a) inv_low_contains r
-
-(** ** Elaboration of the operations **) 
-
-let elab_write (#t:typ0) (r:ref (elab_typ0 t)) (v:elab_typ0 t) 
-: IST unit
-  (requires (fun h0 -> 
-    shallowly_contained_low r #(elab_typ0_tc (TRef t)) h0 /\
-    shallowly_contained_low v #(elab_typ0_tc t) h0))
-  (ensures (fun h0 () h1 ->
-    write_post r v h0 () h1 /\
-    modifies_only_label Low h0 h1 /\
-    shallowly_contained_low r #(elab_typ0_tc (TRef t)) h1))
-= let h0 = get () in
-  write r v;
-  let h1 = get () in
-  lemma_write_preserves_is_low (to_inv_typ t) r v h0 h1;
-  lemma_write_preserves_contains (to_inv_typ t) r v h0 h1;
-  ()
-
-let declassify_low' (#t:typ0) (r:ref (elab_typ0 t)) : ST unit
-  (fun h -> (elab_typ0_tc (TRef t)).satisfy r h contains_pred /\ inv_points_to h contains_pred)
-  (fun h0 () h1 -> 
-    inv_points_to h1 contains_pred /\
-    shallowly_contained_low r #(elab_typ0_tc (TRef t)) h1 /\
-    declassify_post r Low h0 () h1)
-=
-  let h0 = get () in
-  declassify r Low;
-  let h1 = get () in
-  lemma_declassify_preserves_contains (to_inv_typ t) r h0 h1
-
-val elab_alloc (#t:typ0) (init:elab_typ0 t)
-: IST (ref (elab_typ0 t))
-  (requires (fun h0 ->
-    shallowly_contained_low init #(elab_typ0_tc t) h0))
-  (ensures (fun h0 r h1 -> 
-    fresh r h0 h1 /\ 
-    modifies Set.empty h0 h1 /\
-    modifies_classification Set.empty h0 h1 /\
-    sel h1 r == init /\
-    shallowly_contained_low r #(elab_typ0_tc (TRef t)) h1))
-let elab_alloc #t init = 
-  let h0 = get () in
-  let r : ref (elab_typ0 t) = ist_alloc init in
-  let h1 = get () in
-  declassify_low' r;
-  let h2 = get () in
-  (elab_typ0_tc t).satisfy_monotonic init is_low_pred h0 h1;
-  lemma_declassify_preserves_is_low (to_inv_typ t) r h1 h2;
-  assert (inv_points_to h2 is_low_pred);
-  r
-
 (** ** Examples **) 
 
 val ctx_update_ref_test : 
   elab_typ (TArr (TRef TNat) TUnit)
 let ctx_update_ref_test y =
   let y : ref int = downgrade_val y in
-  elab_write #TNat y (!y + 1);
+  sst_write #SNat y (sst_read y + 1);
   raise_val ()
 
 val ctx_update_multiple_refs_test : 
   elab_typ (TArr (TRef (TRef TNat)) (TArr (TRef TNat) TUnit))
 let ctx_update_multiple_refs_test x =
   let x : ref (ref int) = downgrade_val x in
-  mst_witness (contains_pred x);
-  mst_witness (is_low_pred x);
+  witness (contains_pred x);
+  witness (shareS.is_shared x);
   let cb : elab_typ (TArr (TRef TNat) TUnit) = (fun y ->
     let y : ref int = downgrade_val y in
-    let h0 = get () in
-    mst_recall (contains_pred x);
-    let ix : ref int = !x in
-    mst_recall (is_low_pred x);   
-    eliminate_inv_contains' h0 (TRef TNat) x;
-    elab_write #TNat ix (!ix + 1);
-    let h1 = get () in
-    elab_write #(TRef TNat) x y;
-    let h2 = get () in
-    elab_write #TNat y (!y + 5);
-    let h3 = get () in
-    eliminate_inv_low' h0 (TRef TNat) x;
-    lemma_modifies_only_label_trans Low h0 h1 h2;
-    lemma_modifies_only_label_trans Low h0 h2 h3;
-    assert (modifies_only_label Low h0 h3);
-    let r = raise_val () in
-    assert (shallowly_contained_low r h3);
-    assert (inv_low_contains h3);
-    assert (modifies_classification Set.empty h0 h3);
-    r
+    recall (contains_pred x);
+    let ix : ref int = sst_read #(SRef SNat) x in
+    recall (shareS.is_shared x);   
+    sst_write #SNat ix (sst_read ix + 1);
+    sst_write #(SRef SNat) x y;
+    sst_write #SNat y (sst_read y + 5);
+    raise_val () 
   ) in
   cb
 
 val ctx_HO_test1 : 
   elab_typ (TArr (TRef (TPair (TRef TNat) (TRef TNat))) (TArr TUnit TUnit))
 let ctx_HO_test1 xs =
-  let xs : ref ((ref int) * ref int) = downgrade_val xs in
-  let (x', x'') = !xs in
   let h0 = get () in
-  eliminate_inv_contains' h0 (TPair (TRef TNat) (TRef TNat)) xs;
-  eliminate_inv_low' h0 (TPair (TRef TNat) (TRef TNat)) xs;
-  elab_write #(TPair (TRef TNat) (TRef TNat)) xs (x', x');
-  mst_witness (is_low_pred xs);
-  mst_witness (is_low_pred x');
-  mst_witness (is_low_pred x'');
+  let xs : ref ((ref int) * ref int) = downgrade_val xs in
+  let (x', x'') : (ref int) * ref int = sst_read #(SPair (SRef SNat) (SRef SNat)) xs in
+  sst_write #(SPair (SRef SNat) (SRef SNat)) xs (x', x');
+  witness (contains_pred xs); witness (contains_pred x'); witness (contains_pred x'');
+  witness (shareS.is_shared xs); witness (shareS.is_shared x'); witness (shareS.is_shared x'');
   (fun _ -> 
-    mst_recall (is_low_pred xs);
-    mst_recall (is_low_pred x');
-    mst_recall (is_low_pred x'');
-    elab_write #(TPair (TRef TNat) (TRef TNat)) xs (x', x'');
+    recall (contains_pred xs); recall (contains_pred x'); recall (contains_pred x'');
+    recall (shareS.is_shared xs); recall (shareS.is_shared x'); recall (shareS.is_shared x'');
+    sst_write #(SPair (SRef SNat) (SRef SNat)) xs (x', x'');
     raise_val ())
   
 val ctx_identity :
@@ -552,85 +174,71 @@ val ctx_HO_test2 :
 let ctx_HO_test2 f =
   let h0 = get () in
   let x:ref int = downgrade_val (f (raise_val ())) in
-  let h1 = get () in
-  elab_write #TNat x (!x + 1);
-  let h2 = get () in
-  assert (modifies_only_label Low h0 h2);
+  sst_write #SNat x (!x + 1);
   raise_val ()
 
 val ctx_swap_ref_test :
   elab_typ (TArr (TRef (TRef TNat)) (TArr (TRef (TRef TNat)) TUnit))
 let ctx_swap_ref_test x =
   let x : ref (ref int) = downgrade_val x in
-  mst_witness (contains_pred x);
-  mst_witness (is_low_pred x);
+  witness (contains_pred x);
+  witness (shareS.is_shared x);
   let cb : elab_typ (TArr (TRef (TRef TNat)) TUnit) = (fun y ->
     let y : ref (ref int) = downgrade_val y in
-    let h0 = get () in
-    mst_recall (contains_pred x);
-    mst_recall (is_low_pred x);
-    eliminate_inv_contains' h0 (TRef TNat) x;
-    eliminate_inv_low' h0 (TRef TNat) x;
+    recall (contains_pred x);
+    recall (shareS.is_shared x);
     
-    let z = !x in
-    let t = !y in
-    elab_write #(TRef TNat) x t;
-  
-    let h1 = get () in
-    elab_write #(TRef TNat) y z;
-    let h2 = get () in
+    let z = sst_read x in
+    let t = sst_read y in
+    sst_write #(SRef SNat) x t;
+    sst_write #(SRef SNat) y z;
 
-    assert (modifies_classification Set.empty h0 h1);
-    lemma_modifies_only_label_trans Low h0 h1 h2;
-    assert (modifies_only_label Low h0 h2); // we have an SMT Pat for this, but it does not kick in
-    assert (modifies_classification Set.empty h0 h2);
-    assert (inv_low_contains h2);
-    let r = raise_val () in
-    assert (shallowly_contained_low r h2);
-    r) in
+    raise_val ()) in
   cb
 
 val ctx_dynamic_alloc_test :
    elab_typ (TArr TUnit (TRef TNat))
 let ctx_dynamic_alloc_test _ = 
-  let v = elab_alloc #TNat 0 in 
+  let v = sst_alloc_shared #SNat 0 in 
   raise_val v
 
 val ctx_HO_test3 :
   elab_typ (TArr (TArr TUnit (TRef TNat)) TUnit)
 let ctx_HO_test3 f =
   let x:ref int = downgrade_val (f (raise_val ())) in
-  let y:ref int = elab_alloc #TNat (!x + 1) in
+  let y:ref int = sst_alloc_shared #SNat (!x + 1) in
   raise_val ()
 
+#push-options "--split_queries always"
 val ctx_returns_callback_test :
   elab_typ (TArr TUnit (TArr TUnit TUnit))
 let ctx_returns_callback_test _ =
-  let x: ref int = elab_alloc #TNat 13 in
-  mst_witness (contains_pred x);
-  mst_witness (is_low_pred x);
+  let x: ref int = sst_alloc_shared #SNat 13 in
+  witness (contains_pred x);
+  witness (shareS.is_shared x);
   let cb : elab_typ (TArr TUnit TUnit) = (fun _ ->
-    mst_recall (contains_pred x);
-    mst_recall (is_low_pred x);
-    elab_write #TNat x (!x % 5);
+    recall (contains_pred x);
+    recall (shareS.is_shared x);
+    sst_write #SNat x (sst_read x % 5);
     raise_val ()
   ) in
   cb
+#pop-options
 
 val ctx_HO_test4 :
   elab_typ (TArr (TArr TUnit (TRef TNat)) TUnit)
 let ctx_HO_test4 f =
   let x:ref int = downgrade_val (f (raise_val ())) in
-  let y:ref (ref int) = elab_alloc #(TRef TNat) x in
+  let y:ref (ref int) = sst_alloc_shared #(SRef SNat) x in
   raise_val ()
 
 val progr_sep_test: 
   #rp: ref int -> 
   ctx:(elab_typ (TArr TUnit TUnit)) ->
-  IST unit
+  SST unit
     (requires (fun h0 -> 
       satisfy rp h0 contains_pred /\
-      label_of rp h0 == High))
+      ~(shareS.is_shared rp h0)))
     (ensures (fun h0 _ h1 ->
       sel h0 rp == sel h1 rp)) // the content of rp should stay the same before/ after calling the context
          
@@ -640,38 +248,30 @@ let progr_sep_test #rp f = (** If this test fails, it means that the spec of f d
 val progr_declassify :
   rp: ref int -> 
   ctx:(elab_typ (TArr (TRef TNat) TUnit)) ->
-  IST unit
+  SST unit
     (requires (fun h0 -> 
       satisfy rp h0 contains_pred /\
-      label_of rp h0 == High))
+      ~(shareS.is_shared rp h0)))
     (ensures (fun h0 _ h1 -> True))
 let progr_declassify rp f =
   let h0 = get () in
-  declassify_low' #TNat rp;
+  sst_share #SNat rp;
   let h1 = get () in
-  lemma_declassify_preserves_is_low InvT_Nat rp h0 h1;
   let r = downgrade_val (f (raise_val rp)) in  
   r
 
 val progr_declassify_nested:
   rp: ref (ref int) -> 
   ctx:(elab_typ (TArr (TRef (TRef TNat)) TUnit)) ->
-  IST unit
+  SST unit
     (requires (fun h0 -> 
       satisfy rp h0 contains_pred /\
-      label_of rp h0 == High))
+      ~(shareS.is_shared rp h0)))
     (ensures (fun h0 _ h1 -> True))
 let progr_declassify_nested rp f =
-  let h0 = get () in
-  eliminate_inv_contains' h0 (TRef TNat) rp;
-
-  let p : ref int = !rp in
-  declassify_low' #TNat p;
-  let h1 = get () in
-  lemma_declassify_preserves_is_low InvT_Nat p h0 h1;
-  declassify_low' #(TRef TNat) rp;
-  let h2 = get () in
-  lemma_declassify_preserves_is_low (InvT_Ref InvT_Nat) rp h1 h2;
+  let p : ref int = sst_read #(SRef SNat) rp in
+  sst_share #SNat p;
+  sst_share #(SRef SNat) rp;
   // let r = elab_alloc (!rp) in (* <-- needed a copy here! *) 
   downgrade_val (f (raise_val rp))
 
@@ -679,45 +279,43 @@ val progr_secret_unchanged_test:
   rp: ref int -> 
   rs: ref (ref int) ->
   ctx:(elab_typ (TArr TUnit TUnit)) ->
-  IST unit 
+  SST unit 
     (requires (fun h0 -> 
       satisfy rp h0 contains_pred /\
-      label_of rp h0 == High /\
-      satisfy rs h0 is_low_pred))
+      ~(shareS.is_shared rp h0) /\
+      satisfy rs h0 shareS.is_shared))
     (ensures (fun h0 _ h1 ->
       sel h0 rp == sel h1 rp))
          
 let progr_secret_unchanged_test rp rs ctx = 
-  let secret: ref int = ist_alloc #InvT_Nat 0 in
+  let h0 = get () in
+  let secret: ref int = sst_alloc #SNat 0 in
+  let h1 = get () in
   downgrade_val (ctx (raise_val ()));
-  let v = !secret in
-  assert (v == 0);
+  let v = sst_read #SNat secret in
   ()
 
 val progr_passing_callback_test: 
   rp: ref int -> 
   rs: ref (ref int) ->
   ctx:(elab_typ (TArr (TArr TUnit TUnit) TUnit)) ->
-  IST unit 
+  SST unit 
     (requires (fun h0 ->
       satisfy rp h0 contains_pred /\
-      label_of rp h0 == High /\
-      satisfy rs h0 is_low_pred))
+      ~(shareS.is_shared rp h0) /\
+      satisfy rs h0 shareS.is_shared))
     (ensures (fun h0 _ h1 -> sel h0 rp == sel h1 rp)) // the content of rp should stay the same before/ after calling the context
 
 // TODO: the callback of the program should be able to modify rp
 let progr_passing_callback_test rp rs f =
-  let secret: ref int = ist_alloc #InvT_Nat 0 in
-  let h0 = get () in
-  declassify_low' #TNat secret;
-  let h1 = get () in
-  lemma_declassify_preserves_is_low InvT_Nat secret h0 h1;
-  mst_witness (contains_pred secret);
-  mst_witness (is_low_pred secret);
+  let secret: ref int = sst_alloc #SNat 0 in
+  sst_share #SNat secret;
+  witness (contains_pred secret);
+  witness (shareS.is_shared secret);
   let cb: elab_typ (TArr TUnit TUnit) = (fun _ -> 
-    mst_recall (contains_pred secret);
-    mst_recall (is_low_pred secret);
-    elab_write #TNat secret (!secret + 1);
+    recall (contains_pred secret);
+    recall (shareS.is_shared secret);
+    sst_write #SNat secret (!secret + 1);
     raise_val ()) in
   downgrade_val (f cb);
   ()
@@ -726,18 +324,13 @@ val progr_getting_callback_test:
   rp: ref int -> 
   rs: ref (ref int) ->
   ctx:(elab_typ (TArr TUnit (TArr TUnit TUnit))) ->
-  IST unit 
+  SST unit 
     (requires (fun h0 ->
       satisfy rp h0 contains_pred /\
-      label_of rp h0 == High /\
-      satisfy rs h0 is_low_pred))
+      ~(shareS.is_shared rp h0) /\
+      satisfy rs h0 shareS.is_shared))
     (ensures (fun h0 _ h1 -> sel h0 rp == sel h1 rp))
 let progr_getting_callback_test rp rs f =
-  let h0 = get () in
   let cb = f (raise_val ()) in
-  let h1 = get () in
   downgrade_val (cb (raise_val ()));
-  let h2 = get () in
-  lemma_modifies_only_label_trans Low h0 h1 h2;
-  assert (modifies_only_label Low h0 h2);
   ()
